compiler/src/examples/Fibonacci.v
@@ -1,13 +1,12 @@
 Require Import Coq.Lists.List.
 Import ListNotations.
 Require Import lib.LibTacticsMin.
-Require Import bbv.WordScope.
+Require Import riscv.util.Word.
 Require Import compiler.Decidable.
 Require Import compiler.Op.
 Require Import compiler.ExprImp.
 Require Import compiler.NameGen.
 Require Import compiler.Pipeline.
-Require Import riscv.Riscv.
 Require Import compiler.util.MyOmega.
 Require Import riscv.util.Monads.
 Require Import compiler.util.Common.
@@ -17,7 +16,7 @@ Require        riscv.InstructionNotations.
 Require Import riscv.ListMemory.
 Require Import riscv.MinimalLogging.
 Require Import riscv.Utility.
-Require Import riscv.encode.Encode.
+Require Import riscv.Encode.
 Require Import compiler.ZName.
 Require Import riscv.util.BitWidth32.
 Require Import riscv.MachineWidth32.
@@ -30,6 +29,8 @@ Open Scope Z_scope.
 
 Definition var: Set := (@name ZName).
 Definition Reg: Set := (@name ZName).
+
+Existing Instance MachineWidth32.MachineWidth32.
 
 Existing Instance DefaultRiscvState.
 
@@ -51,45 +52,47 @@ while i < n:
   i = i + 1
 *)
 
-Definition fib_ExprImp(n: word wXLEN): stmt :=
-  SSeq (SSet var_a (ELit $0)) (
-  SSeq (SSet var_b (ELit $1)) (
-  SSeq (SSet var_i (ELit $0)) (
+Definition ELit(x: Z): expr := ELit (ZToWord XLEN x).
+
+Definition fib_ExprImp(n: Z): stmt :=
+  SSeq (SSet var_a (ELit 0)) (
+  SSeq (SSet var_b (ELit 1)) (
+  SSeq (SSet var_i (ELit 0)) (
   SWhile (EOp OLt (EVar var_i) (ELit n)) (
     SSeq (SSet var_c (EOp OPlus (EVar var_a) (EVar var_b))) (
     SSeq (SSet var_a (EVar var_b)) (
     SSeq (SSet var_b (EVar var_c)) (
-    SSeq (SSet var_i (EOp OPlus (EVar var_i) (ELit $1)))
+    SSeq (SSet var_i (EOp OPlus (EVar var_i) (ELit 1)))
     SSkip))))))).
 
-Definition state := (var -> option (word wXLEN)).
+Definition state := (var -> option (word XLEN)).
 
 Instance fooo: MapFunctions name (list name * list name * stmt (mword := word 32)). Admitted.
 
-Definition fib_H_res(fuel: nat)(n: word wXLEN): option (word wXLEN) :=
+Definition fib_H_res(fuel: nat)(n: Z): option (word 32) :=
   match (eval_stmt empty_map fuel empty_map Memory.no_mem (fib_ExprImp n)) with
-  | Some (st, m) => get st var_b
+  | Some (st, m) => Map.get st var_b
   | None => None
   end.
 
 
-Goal fib_H_res 20 $0 = Some $1. reflexivity. Qed.
-Goal fib_H_res 20 $1 = Some $1. reflexivity. Qed.
-Goal fib_H_res 20 $2 = Some $2. reflexivity. Qed.
-Goal fib_H_res 20 $3 = Some $3. reflexivity. Qed.
-Goal fib_H_res 20 $4 = Some $5. reflexivity. Qed.
-Goal fib_H_res 20 $5 = Some $8. reflexivity. Qed.
-Goal fib_H_res 20 $6 = Some $13. reflexivity. Qed.
+Goal fib_H_res 20 0 = Some (ZToWord 32  1). reflexivity. Qed.
+Goal fib_H_res 20 1 = Some (ZToWord 32  1). reflexivity. Qed.
+Goal fib_H_res 20 2 = Some (ZToWord 32  2). reflexivity. Qed.
+Goal fib_H_res 20 3 = Some (ZToWord 32  3). reflexivity. Qed.
+Goal fib_H_res 20 4 = Some (ZToWord 32  5). reflexivity. Qed.
+Goal fib_H_res 20 5 = Some (ZToWord 32  8). reflexivity. Qed.
+Goal fib_H_res 20 6 = Some (ZToWord 32 13). reflexivity. Qed.
 
 Definition do_regalloc: bool := false.
 
 Definition compileFunc: stmt -> list Instruction :=
   if do_regalloc then (exprImp2Riscv_with_regalloc Lw Sw) else (exprImp2Riscv Lw Sw).
 
-Definition fib_riscv0(n: word wXLEN): list Instruction :=
+Definition fib_riscv0(n: Z): list Instruction :=
   compileFunc (fib_ExprImp n).
 
-Definition fib6_riscv := Eval cbv in fib_riscv0 $6.
+Definition fib6_riscv := Eval cbv in fib_riscv0 6.
 
 Print fib6_riscv.
 
@@ -97,17 +100,40 @@ Import riscv.InstructionNotations.
 
 Print fib6_riscv.
 
+Goal forall a, ZToWord 2 1 = a.
+  intros.
+  unfold ZToWord.
+  cbv.
+  (* TODO cbv trying to reduce the first argument of exist is bad... *)
+Abort.
+
+(* TODO make this work
+Eval cbv in (ZToWord 32 2523456327).
+
+as fast as this one:
+Require bbv.Word.
+Eval cbv in (bbv.Word.ZToWord 32 2523456327).
+
+*)
+
 Definition fib6_bits: list (word 32) :=
   List.map (fun i => ZToWord 32 (encode i)) fib6_riscv.
 
+(* TODO after above TODO, this should work again
 Eval cbv in fib6_bits.
+*)
+
+Definition fib6_bits_as_Z: list Z :=
+  List.map (fun i => (encode i)) fib6_riscv.
+
+Eval cbv in fib6_bits_as_Z.
 
 (* This example uses the memory only as instruction memory
    TODO make an example which uses memory to store data *)
 Definition zeroedRiscvMachineCore: RiscvMachineCore := {|
   registers := initialRegs;
-  pc := $0;
-  nextPC := (natToWord 32 4);
+  pc := ZToWord 32 0;
+  nextPC := (ZToWord 32 4);
   exceptionHandlerAddr := 3;
 |}.
 
@@ -117,7 +143,7 @@ Definition zeroedRiscvMachine: RiscvMachine := {|
 |}.
 
 Definition initialRiscvMachine(imem: list (word 32)): RiscvMachine :=
-  Minimal.putProgram imem $0 zeroedRiscvMachine.
+  Minimal.putProgram imem (ZToWord 32 0) zeroedRiscvMachine.
 
 Definition zeroedRiscvMachineL: RiscvMachineL := {|
     machine := zeroedRiscvMachine;
@@ -125,7 +151,7 @@ Definition zeroedRiscvMachineL: RiscvMachineL := {|
 |}.
 
 Definition initialRiscvMachineL(imem: list (word 32)): RiscvMachineL :=
-  putProgram imem $0 zeroedRiscvMachineL.
+  putProgram imem (ZToWord 32 0) zeroedRiscvMachineL.
 
 Definition run: nat -> RiscvMachine -> option unit * RiscvMachine :=
  @Run.run BitWidth32 _ MachineWidth32 (OState RiscvMachine) (OState_Monad _) _ _  .
@@ -139,17 +165,17 @@ Definition fib6_L_final(fuel: nat): RiscvMachine :=
 Definition fib6_L_finalL(fuel: nat): RiscvMachineL :=
   snd (runL fuel (initialRiscvMachineL fib6_bits)).
 
-Definition force_option(o: option (word wXLEN)): word wXLEN :=
+Definition force_option(o: option (word XLEN)): word XLEN :=
   match o with
   | Some w => w
-  | None => $0
+  | None => ZToWord XLEN 0
   end.
 
-Definition fib6_L_res(fuel: nat): word wXLEN :=
-  force_option (get (fib6_L_final fuel).(core).(registers) var_b).
+Definition fib6_L_res(fuel: nat): word XLEN :=
+  force_option (Map.get (fib6_L_final fuel).(core).(registers) var_b).
 
-Definition fib6_L_resL(fuel: nat): word wXLEN :=
-  force_option (get (fib6_L_finalL fuel).(machine).(core).(registers) var_b).
+Definition fib6_L_resL(fuel: nat): word XLEN :=
+  force_option (Map.get (fib6_L_finalL fuel).(machine).(core).(registers) var_b).
 
 Definition fib6_L_trace(fuel: nat): Log :=
   (fib6_L_finalL fuel).(log).
@@ -161,7 +187,8 @@ Definition fib6_L_trace(fuel: nat): Log :=
 Eval cbv in (fib6_L_trace 1000).
 Eval cbv in (length (fib6_L_trace 1000)).
 
-Eval cbv in (fib6_L_res 400).
+(* TODO remove surrounding uwordToZ *)
+Eval cbv in (uwordToZ (fib6_L_res 400)).
 
 (* If cbv and vm_compute block or better performance is needed, we can extract to Haskell:
 Definition finalfibres: nat := wordToNat (fib6_L_res 400).
@@ -169,30 +196,32 @@ Require Extraction.
 Extraction Language Haskell.
 Set Warnings "-extraction-reserved-identifier".
 Extraction "Fib6.hs" finalfibres.
-*)
+ *)
 
 (* 1st method: Run it *)
-Lemma fib6_L_res_is_13_by_running_it: exists fuel, fib6_L_res fuel = $13.
+Lemma fib6_L_res_is_13_by_running_it: exists fuel, uwordToZ (fib6_L_res fuel) = 13.
   exists 400%nat.
   cbv.
   reflexivity.
 Qed.
 
-Lemma fib_H_res_value: fib_H_res 20 $6 = Some $13.
+Lemma fib_H_res_value: fib_H_res 20 6 = Some (ZToWord 32 13).
+Admitted. (* TODO
 Proof. cbv. reflexivity. Qed.
+           *)
 
-Lemma enough_registers_for_fib6: enough_registers (fib_ExprImp $6).
+Lemma enough_registers_for_fib6: enough_registers (fib_ExprImp 6).
 Proof.
   cbv. auto 20.
 Qed.
 
 (* 2nd method: Prove it without running it on low level, but using the
    compiler correctness theorem *)
-Lemma fib6_L_res_is_13_by_proving_it: exists fuel, fib6_L_res fuel = $13.
+Lemma fib6_L_res_is_13_by_proving_it: exists fuel, uwordToZ (fib6_L_res fuel) = 13.
   unfold fib6_L_res. unfold fib6_L_final.
   pose proof @exprImp2Riscv_correct as P.
   assert (exists finalH,
-             evalH Lw Sw empty_map 20 empty_map Memory.no_mem (fib_ExprImp $ (6)) = Some finalH) as F. {
+             evalH Lw Sw empty_map 20 empty_map Memory.no_mem (fib_ExprImp 6) = Some finalH) as F. {
     eexists. reflexivity.
   }
   destruct F as [ [finalH finalMH ] F ].
@@ -227,6 +256,8 @@ Lemma fib6_L_res_is_13_by_proving_it: exists fuel, fib6_L_res fuel = $13.
     unfold force_option, run, fib6_bits, initialRiscvMachine.
     unfold getReg, FlatToRiscv.State_is_RegisterFile, Map.get, List_Map in G.
     unfold evalL, execState in G.
+Admitted.
+(*
     apply G. clear G.
     assert (forall T (a b: T), Some a = Some b -> a = b) as E. {
       introv R. inversion R. reflexivity.
@@ -239,5 +270,6 @@ Lemma fib6_L_res_is_13_by_proving_it: exists fuel, fib6_L_res fuel = $13.
     end.
     assumption.
 Qed.    
+*)
 
 Print Assumptions fib6_L_res_is_13_by_proving_it.
