compiler/src/examples/TestExprImp.v
@@ -1,5 +1,5 @@
 Require Import lib.LibTacticsMin.
-Require Import bbv.WordScope.
+Require Import riscv.util.Word.
 Require Import riscv.util.BitWidths.
 Require Import compiler.util.Common.
 Require Import compiler.util.Tactics.
@@ -52,14 +52,17 @@ Definition annoying_eq: DecidableEq
   (list (@name ZName) * list (@name ZName) * @stmt (word 32) ZName ZName). Admitted.
 Existing Instance annoying_eq.
 
-Definition run_isRight(x y z: word 32): option (word 32) :=
+Definition run_isRight(xz yz zz: Z): option (word 32) :=
+  let x := ZToWord 32 xz in
+  let y := ZToWord 32 yz in
+  let z := ZToWord 32 zz in
   final <- (eval_stmt empty_map 10 empty_map no_mem (isRight x y z));
   let '(finalSt, finalM) := final in
   get finalSt _isRight.
 
-Goal run_isRight $3 $4 $5 = Some $1. reflexivity. Qed.
-Goal run_isRight $3 $7 $5 = Some $0. reflexivity. Qed.
-Goal run_isRight $4 $3 $5 = Some $1. reflexivity. Qed.
-Goal run_isRight $5 $3 $5 = Some $0. reflexivity. Qed.
-Goal run_isRight $5 $3 $4 = Some $1. reflexivity. Qed.
-Goal run_isRight $12 $13 $5 = Some $1. reflexivity. Qed.
+Goal run_isRight  3  4  5 = Some (ZToWord 32 1). reflexivity. Qed.
+Goal run_isRight  3  7  5 = Some (ZToWord 32 0). reflexivity. Qed.
+Goal run_isRight  4  3  5 = Some (ZToWord 32 1). reflexivity. Qed.
+Goal run_isRight  5  3  5 = Some (ZToWord 32 0). reflexivity. Qed.
+Goal run_isRight  5  3  4 = Some (ZToWord 32 1). reflexivity. Qed.
+Goal run_isRight 12 13  5 = Some (ZToWord 32 1). reflexivity. Qed.
